pico-ifc-coq/basic_machines/CLabels.v
@@ -1,0 +1,49 @@
+Require Import ZArith.
+Require Import List.
+
+Require Import Instr.
+Require Import CodeSpecs.
+Require Import CodeTriples.
+Require Import Concrete.
+Require Import Encodable.
+Require Import Utils.
+
+Definition listify_apply_rule {T} `{Encodable T} (ar: option (T * T)) (s0: stack): stack :=
+  match ar with
+  | None            => CData (0, handlerTag) :: s0
+  | Some (lrpc, lr) => CData (1, handlerTag) ::
+                        CData (labToZ lr, handlerTag) ::
+                        CData (labToZ lrpc, handlerTag) :: s0
+  end.
+
+Definition handler_initial_mem_matches
+           (opcode: Z) (tags : Z * Z * Z)
+           (pctag: Z)
+           (m: memory) : Prop :=
+  let '(tag1,tag2,tag3) := tags in
+     index_list_Z addrOpLabel m = Some (opcode,handlerTag)
+  /\ index_list_Z addrTag1 m = Some (tag1,handlerTag)
+  /\ index_list_Z addrTag2 m = Some (tag2,handlerTag)
+  /\ index_list_Z addrTag3 m = Some (tag3,handlerTag)
+  /\ index_list_Z addrTagPC m = Some (pctag,handlerTag).
+
+Class ConcreteLabels (L : Type)
+                     (EL : Encodable L)
+                     (labelCount : OpCode -> nat)
+                     (run_tmr : forall opcode,
+                                  L ->
+                                  Vector.t L (labelCount opcode) ->
+                                  option (L * L)) := {
+
+  genRule : OpCode -> list Instr;
+
+  genRuleCorrect :
+    forall opcode m0 (labs : Vector.t L (labelCount opcode)) pcl (Q : memory -> stack -> Prop),
+      handler_initial_mem_matches (opCodeToZ opcode) (labsToZs labs) (labToZ pcl) m0 ->
+      HT (genRule opcode)
+         (fun m s =>
+            m = m0 /\
+            Q m (listify_apply_rule (run_tmr opcode pcl labs) s))
+         Q
+
+}.
